examples/MutableBtree.dfy
@@ -791,6 +791,7 @@ abstract module MutableBtree {
     root.repr := {root, rootkeys, rootvalues};
     root.height := 0;
   }
+
 }
 
 module TestBtreeSpec refines BtreeSpec {
