lib/Base/total_order.i.dfy
@@ -678,7 +678,7 @@ abstract module Total_Order {
   
   predicate {:opaque} SortedSeqForMap<V>(s: seq<(Element, V)>, m: map<Element, V>)
   {
-    && (forall i, j :: 0 <= i < j < |s| ==> lt(s[i].0, s[j].0))
+    && IsStrictlySorted(Seq.Unzip(s).0)
     && (forall i :: 0 <= i < |s| ==> s[i].0 in m && m[s[i].0] == s[i].1)
     && (forall key :: key in m ==> (exists i :: 0 <= i < |s| && s[i].0 == key && s[i].1 == m[key]))
   }
